练习 2.24
===============

表达式 ``(list 1 (list 2 (list 3 4)))`` 的打印结果如下：

::

    1 ]=> (list 1 (list 2 (list 3 4)))

    ;Value 11: (1 (2 (3 4)))

它的盒子图形如下：

::

     (1 (2 (3 4)))       ((2 (3 4)))
    [*]---------------> [*]
     |                   |
     |                   |
     v                   v (2 (3 4))         ((3 4))
     1                  [*]---------------> [*]
                         |                   |
                         |                   |
                         v                   v (3 4)             (4)          
                         2                  [*]---------------> [*]---------------> '()
                                             |                   |
                                             |                   |
                                             v                   v
                                             3                   4

它的树图形如下：

::

     (1 (2 (3 4)))
       *
      / \
     /   \  (2 (3 4))
    1     *
         / \
        /   \  (3 4)
       2     *
            / \
           /   \ 
          3     4
